new/proof/go_etcd_io/etcd/client/v3/leasing.v
@@ -2,3 +2,5 @@ Require Import New.code.go_etcd_io.etcd.client.v3.leasing.
 Require Import New.generatedproof.go_etcd_io.etcd.client.v3.leasing.
 Require Import New.proof.proof_prelude.
 Require Import New.proof.context.
+
+Require Import New.proof.go_etcd_io.etcd.client.v3.concurrency.
